wip (admits in safe and open)

ems/Skeleton.v
@@ -76,17 +76,22 @@ Module Sk.
     unit: t;
     add: t -> t -> t;
     canon: t -> sem;
-    wf: t -> Prop;
+    wf: sem -> Prop;
     add_comm: forall a b,
       canon (add a b) = canon (add b a);
     add_assoc: forall a b c,
       canon (add a (add b c)) = canon (add (add a b) c);
     add_unit_l: forall a, canon (add unit a) = canon a;
     add_unit_r: forall a, canon (add a unit) = canon a;
-    wf_comm: forall a b, wf (add a b) -> wf (add b a);
-    unit_wf: wf unit;
-    wf_mon: forall a b, wf (add a b) -> wf a;
-    extends := fun a b => exists ctx, canon (add a ctx) = b;
+    (* wf_comm: forall a b, wf (add a b) -> wf (add b a);
+    wf_assoc: forall a b c, wf (add a (add b c)) <-> wf (add (add a b) c); *)
+    add_canon: forall a b a' b',
+      canon a = canon a' ->
+        canon b = canon b' ->
+          canon (add a b) = canon (add a' b');
+    unit_wf: wf (canon unit);
+    wf_mon: forall a b, wf (canon (add a b)) -> wf (canon a);
+    extends := fun a b => exists ctx, canon (add a ctx) = canon b;
   }
   .
 
@@ -104,11 +109,12 @@ Module Sk.
 
   Program Instance globalenv : ld := {
     t := PTree.t RA.car;
-    sem := alist string RA.car;
+    sem := alist positive RA.car;
     unit := PTree.empty RA.car;
     add := PTree.combine _add;
-    canon:= (List.map (map_fst string_of_ident)) ∘ (@PTree.elements RA.car);
-    wf := fun m => forall p x, PTree.get p m = Some x -> RA.wf x;
+    canon:= @PTree.elements RA.car;
+    wf := fun m => forall s x, alist_find s m = Some x -> RA.wf x
+                   /\ NoDup (map (map_fst string_of_ident) m);
   }.
   Next Obligation.
   Proof.
@@ -117,114 +123,100 @@ Module Sk.
   Qed.
   Next Obligation.
   Proof.
-    f_equal. apply PTree.elements_extensional.
+    apply PTree.elements_extensional.
     i. repeat (rewrite PTree.gcombine; et).
     unfold _add. des_ifs. f_equal. apply RA.add_assoc.
   Qed.
   Next Obligation.
   Proof.
-    f_equal. apply PTree.elements_extensional.
+    apply PTree.elements_extensional.
     i. rewrite PTree.xgcombine_r; et.
     unfold _add. des_ifs.
   Qed.
   Next Obligation.
   Proof.
-    f_equal. apply PTree.elements_extensional.
+    apply PTree.elements_extensional.
     i. repeat (rewrite PTree.gcombine; et).
     unfold _add. des_ifs.
     all: rewrite PTree.gempty in Heq0; clarify.
   Qed.
+  (* Next Obligation.
+  Proof.
+    split.
+    - erewrite PTree.combine_commut in H0; try eapply H; et.
+      i. unfold _add. des_ifs. f_equal. apply RA.add_comm.
+    - admit.
+  Admitted.
   Next Obligation.
   Proof.
-    erewrite PTree.combine_commut in H0; try eapply H; et.
-    i. unfold _add. des_ifs. f_equal. apply RA.add_comm.
-  Qed.
+  Admitted. *)
   Next Obligation.
   Proof.
-    rewrite PTree.gempty in H. ss.
-  Qed.
+  Admitted.
   Next Obligation.
   Proof.
-    specialize (H p). rewrite PTree.gcombine in H; et.
-    rewrite H0 in H. destruct (b ! p).
-    - hexploit H; et. eapply RA.wf_mon.
-    - hexploit H; et.
-  Qed.
+    split. 2:{ admit. }
+    (* apply PTree.elements_extensional.
+    i. repeat (rewrite PTree.gcombine; et).
+    f_equal.
+    - destruct (a ! i) eqn: E; destruct (a' ! i) eqn: E'; et.
+      + apply PTree.elements_correct in E. rewrite H in E.
+        apply PTree.elements_complete in E. clarify.
+      + apply PTree.elements_correct in E. rewrite H in E.
+        apply PTree.elements_complete in E. clarify.
+      + apply PTree.elements_correct in E'. rewrite <- H in E'.
+        apply PTree.elements_complete in E'. clarify.
+    - destruct (b ! i) eqn: E; destruct (b' ! i) eqn: E'; et.
+      + apply PTree.elements_correct in E. rewrite H0 in E.
+        apply PTree.elements_complete in E. clarify.
+      + apply PTree.elements_correct in E. rewrite H0 in E.
+        apply PTree.elements_complete in E. clarify.
+      + apply PTree.elements_correct in E'. rewrite <- H0 in E'.
+        apply PTree.elements_complete in E'. clarify. *)
+  Admitted.
 
-  Local Existing Instance gdefs.
-
-  Definition sort_add_comm sk0 sk1
-             (WF: wf (add sk0 sk1))
-    :
-      sort (add sk0 sk1) = sort (add sk1 sk0).
-  Proof.
-    eapply SkSort.sort_add_comm. eapply WF.
-  Qed.
-
-  Definition sort_wf sk (WF: wf sk):
-    wf (sort sk).
-  Proof.
-    ss. eapply Permutation.Permutation_NoDup; [|apply WF].
-    eapply Permutation.Permutation_map.
-    eapply SkSort.sort_permutation.
-  Qed.
+  Local Existing Instance globalenv.
 
   (*** TODO: It might be nice if Sk.t also constitutes a resource algebra ***)
   (*** At the moment, List.app is not assoc/commutative. We need to equip RA with custom equiv. ***)
 
-  Definition load_skenv (sk: t): (SkEnv.t) :=
-    let n := List.length sk in
+  Definition load_skenv (sks: sem): (SkEnv.t) :=
     {|
-      SkEnv.blk2id := fun blk => do '(gn, _) <- (List.nth_error sk blk); Some gn;
-      SkEnv.id2blk := fun id => do '(blk, _) <- find_idx (fun '(id', _) => string_dec id id') sk; Some blk
+      SkEnv.blk2id := fun blk => do '(id, _) <- (List.nth_error sks blk); Some (string_of_ident id);
+      SkEnv.id2blk := fun gn => do '(blk, _) <- find_idx (fun '(id', _) => dec (ident_of_string gn) id') sks; Some blk
     |}
   .
 
   Lemma load_skenv_wf
-        sk
-        (WF: wf sk)
+        sks
+        (WF: wf sks)
     :
-      <<WF: SkEnv.wf (load_skenv sk)>>
+      <<WF: SkEnv.wf (load_skenv sks)>>
   .
   Proof.
-    r in WF.
-    rr. split; i; ss.
-    - uo; des_ifs.
-      + f_equal. ginduction sk; ss. i. inv WF.
-        rewrite find_idx_red in Heq1. des_ifs; ss.
-        { des_sumbool. subst. ss. clarify. }
-        des_sumbool. uo. des_ifs. destruct p. ss.
-        hexploit IHsk; et.
-      + exfalso. ginduction sk; ss. i. inv WF.
-        rewrite find_idx_red in Heq2. des_ifs; ss.
-        des_sumbool. uo. des_ifs. destruct p. ss.
-        hexploit IHsk; et.
-    - ginduction sk; ss.
-      { i. uo. ss. destruct blk; ss. }
-      i. destruct a. inv WF. uo. destruct blk; ss; clarify.
-      {  rewrite find_idx_red. uo. des_ifs; des_sumbool; ss. }
-      hexploit IHsk; et. i.
-      rewrite find_idx_red. uo. des_ifs; des_sumbool; ss. exfalso.
-      subst. clear - Heq1 H2. ginduction sk; ss. i.
-      rewrite find_idx_red in Heq1. des_ifs; des_sumbool; ss; et.
-      uo. des_ifs. destruct p. eapply IHsk; et.
-  Qed.
+    red. split; i; ss.
+    - uo. des_ifs.
+      + admit.
+      + admit.
+    - uo. des_ifs.
+      + admit.
+      + admit.
+  Admitted.
 
-  Definition incl (sk0 sk1: Sk.t): Prop :=
-    forall gn gd (IN: List.In (gn, gd) sk0),
-      List.In (gn, gd) sk1.
-
-  Program Instance incl_PreOrder: PreOrder incl.
+  Program Instance incl_PreOrder: PreOrder extends.
   Next Obligation.
   Proof.
-    ii. ss.
+    ii. unfold extends. eexists unit. apply add_unit_r.
   Qed.
   Next Obligation.
   Proof.
-    ii. eapply H0. eapply H. ss.
+    ii. unfold extends in *. des. 
+    exists (add ctx0 ctx). rewrite add_assoc.
+    rewrite <- H0.
+    apply add_canon; et.
   Qed.
 
-  Lemma sort_incl sk
+  (* Lemma sort_incl sk
     :
       incl sk (sort sk).
   Proof.
@@ -238,70 +230,51 @@ Module Sk.
   Proof.
     ii. eapply Permutation.Permutation_in; [|apply IN].
     symmetry. eapply SkSort.sort_permutation.
-  Qed.
+  Qed. *)
 
   Definition incl_env (sk0: Sk.t) (skenv: SkEnv.t): Prop :=
-    forall gn gd (IN: List.In (gn, gd) sk0),
+    forall gn gd (IN: sk0 ! (ident_of_string gn) = Some gd),
     exists blk, <<FIND: skenv.(SkEnv.id2blk) gn = Some blk>>.
 
   Lemma incl_incl_env sk0 sk1
-        (INCL: incl sk0 sk1)
+        (INCL: extends sk0 sk1)
     :
-      incl_env sk0 (load_skenv sk1).
+      incl_env sk0 (load_skenv (canon sk1)).
   Proof.
-    ii. exploit INCL; et. i. ss. uo. des_ifs; et.
-    exfalso. clear - x0 Heq0. ginduction sk1; et.
-    i. ss. rewrite find_idx_red in Heq0. des_ifs.
-    des_sumbool. uo.  des_ifs. des; clarify.
-    eapply IHsk1; et.
-  Qed.
+    ii. unfold extends in *. des. rewrite <- INCL.
+    ss. uo. des_ifs; et. 
+    exfalso. clear - IN Heq0. 
+  Admitted.
 
   Lemma in_env_in_sk :
     forall sk blk symb
-      (FIND: SkEnv.blk2id (Sk.load_skenv sk) blk = Some symb),
-    exists def, In (symb, def) sk.
+      (FIND: SkEnv.blk2id (load_skenv (canon sk)) blk = Some symb),
+    exists def, sk ! (ident_of_string symb) = Some def.
   Proof.
-    i. unfold SkEnv.blk2id. ss.
-    uo. des_ifs. des; clarify.
-    eapply nth_error_In in Heq0. et.
-  Qed.
+  Admitted.
+
 
   Lemma in_sk_in_env :
-    forall sk def symb
-           (IN: In (symb, def) sk),
-    exists blk, SkEnv.blk2id (Sk.load_skenv sk) blk = Some symb.
+    forall sk def gn
+           (IN: sk ! (ident_of_string gn) = Some def),
+    exists blk, SkEnv.blk2id (load_skenv (canon sk)) blk = Some gn.
   Proof.
-    i. unfold SkEnv.blk2id. ss.
-    uo. eapply In_nth_error in IN. des.
-    eexists. rewrite IN. et.
-  Qed.
+  Admitted.
 
   Lemma env_range_some :
-    forall sk blk
-      (BLKRANGE : blk < Datatypes.length sk),
-      <<FOUND : exists symb, SkEnv.blk2id (Sk.load_skenv sk) blk = Some symb>>.
+    forall sks blk
+      (BLKRANGE : blk < Datatypes.length sks),
+      <<FOUND : exists symb, SkEnv.blk2id (load_skenv sks) blk = Some symb>>.
   Proof.
-    i. depgen sk. induction blk; i; ss; clarify.
-    { destruct sk; ss; clarify.
-      { lia. }
-      uo. destruct p. exists s. ss. }
-    destruct sk; ss; clarify.
-    { lia. }
-    apply lt_S_n in BLKRANGE. eapply IHblk; eauto.
-  Qed.
+  Admitted.
 
   Lemma env_found_range :
-    forall sk symb blk
-      (FOUND : SkEnv.id2blk (Sk.load_skenv sk) symb = Some blk),
-      <<BLKRANGE : blk < Datatypes.length sk>>.
+    forall sks symb blk
+      (FOUND : SkEnv.id2blk (load_skenv sks) symb = Some blk),
+      <<BLKRANGE : blk < Datatypes.length sks>>.
   Proof.
-    induction sk; i; ss; clarify.
-    uo; des_ifs. destruct p0. rewrite find_idx_red in Heq0. des_ifs.
-    { apply Nat.lt_0_succ. }
-    destruct blk.
-    { apply Nat.lt_0_succ. }
-    uo. des_ifs. destruct p. ss. clarify. apply lt_n_S. eapply IHsk; eauto.
-    instantiate (1:=symb). rewrite Heq0. ss.
-  Qed.
+  Admitted.
+
+End SK.
 
 End Sk.
