spc/Hoare.v
@@ -56,19 +56,20 @@ Qed.
 Section CANCELSTB.
 
   Context `{Σ: GRA.t}.
+  Context `{X: Sk.ld}.
 
   Variable mds: list SMod.t.
 
-  Let sk: Sk.t := SMod.get_sk mds.
+  Let sk: Sk.sem := SMod.get_sk mds.
 
-  Let _mss: Sk.t -> list SModSem.t := fun sk => (List.map ((flip SMod.get_modsem) sk) mds).
-  Let _sbtb: Sk.t -> list (gname * fspecbody) := fun sk => (List.flat_map (SModSem.fnsems) (_mss sk)).
-  Let _stb: Sk.t -> list (gname * fspec) := fun sk => List.map (fun '(fn, fs) => (fn, fs.(fsb_fspec))) (_sbtb sk).
+  Let _mss: Sk.sem -> list SModSem.t := fun sk => (List.map ((flip SMod.get_modsem) sk) mds).
+  Let _sbtb: Sk.sem -> list (gname * fspecbody) := fun sk => (List.flat_map (SModSem.fnsems) (_mss sk)).
+  Let _stb: Sk.sem -> list (gname * fspec) := fun sk => List.map (fun '(fn, fs) => (fn, fs.(fsb_fspec))) (_sbtb sk).
 
   Let mss: list SModSem.t := _mss sk.
   Let sbtb: list (gname * fspecbody) := _sbtb sk.
 
-  Variable stb: Sk.t -> gname -> option fspec.
+  Variable stb: Sk.sem -> gname -> option fspec.
   Hypothesis STBCOMPLETE:
     forall fn fsp (FIND: alist_find fn (_stb sk) = Some fsp), stb sk fn = Some fsp.
   Hypothesis STBSOUND:
@@ -146,12 +147,13 @@ End CANCELSTB.
 Section CANCEL.
 
   Context `{Σ: GRA.t}.
+  Context `{X: Sk.ld}.
 
   Variable mds: list SMod.t.
 
-  Let sk: Sk.t := SMod.get_sk mds.
-  Let stb0: Sk.t -> gname -> option fspec := fun sk => to_stb (SMod.get_stb mds sk).
-  Let stb1: Sk.t -> gname -> option fspec := fun sk => to_closed_stb (SMod.get_stb mds sk).
+  Let sk: Sk.sem := SMod.get_sk mds.
+  Let stb0: Sk.sem -> gname -> option fspec := fun sk => to_stb (SMod.get_stb mds sk).
+  Let stb1: Sk.sem -> gname -> option fspec := fun sk => to_closed_stb (SMod.get_stb mds sk).
 
   Let mds_src: list Mod.t := List.map (SMod.to_src) mds.
   Let mds_tgt0: list Mod.t := List.map (SMod.to_tgt stb0) mds.
@@ -263,17 +265,18 @@ Require Import ClassicalChoice.
 Section CANCEL.
 
   Context `{Σ: GRA.t}.
+  Context `{X: Sk.ld}.
 
   Variable mds: list SMod.t.
 
 
-  Let sk: Sk.t := SMod.get_sk mds.
+  Let sk: Sk.sem := SMod.get_sk mds.
   (* Let sk: Sk.t := Sk.sort (fold_right Sk.add Sk.unit (List.map SMod.sk mds)). *)
   (* Let skenv: SkEnv.t := Sk.load_skenv sk. *)
 
-  Let _mss: Sk.t -> list SModSem.t := fun sk => (List.map ((flip SMod.get_modsem) sk) mds).
-  Let _sbtb: Sk.t -> list (gname * fspecbody) := fun sk => (List.flat_map (SModSem.fnsems) (_mss sk)).
-  Let _stb: Sk.t -> list (gname * fspec) := fun sk => List.map (fun '(fn, fs) => (fn, fs.(fsb_fspec))) (_sbtb sk).
+  Let _mss: Sk.sem -> list SModSem.t := fun sk => (List.map ((flip SMod.get_modsem) sk) mds).
+  Let _sbtb: Sk.sem -> list (gname * fspecbody) := fun sk => (List.flat_map (SModSem.fnsems) (_mss sk)).
+  Let _stb: Sk.sem -> list (gname * fspec) := fun sk => List.map (fun '(fn, fs) => (fn, fs.(fsb_fspec))) (_sbtb sk).
 
   Let mss: list SModSem.t := _mss sk.
   Let sbtb: list (gname * fspecbody) := _sbtb sk.
