spc/Safe.v
@@ -85,11 +85,12 @@ Module SafeMod.
 Section SAFEMOD.
   Context `{EMSConfig}.
   Context `{Σ: GRA.t}.
+  Context `{X: Sk.ld}.
 
   Variable stb: gname -> Prop.
 
   Record t: Type := mk {
-    get_modsem: Sk.t -> SafeModSem.t;
+    get_modsem: Sk.sem -> SafeModSem.t;
     sk: Sk.t;
   }
   .
@@ -106,6 +107,7 @@ Coercion SafeMod.to_smod: SafeMod.t >-> SMod.t.
 
 Section LEMMAS.
   Context `{EMSConfig}.
+  Context `{X: Sk.ld}.
 
   Variable prog: ModL.t.
   Let L := ModL.compile prog.
@@ -234,6 +236,7 @@ Hint Resolve safe_bind_clo_mon: paco.
 Section SAFETY.
   Context `{EMSConfig}.
   Context `{Σ: GRA.t}.
+  Context `{X: Sk.ld}.
 
   Variable smds: list SafeMod.t.
   Variable stb: gname -> Prop.
@@ -266,7 +269,7 @@ Section SAFETY.
   Proof.
     unfold ModL.enclose, mds. unfold Sk.canon. ss.
     change (alist string Any.t) with Sk.t.
-    generalize (Sk.sort (ModL.sk (Mod.add_list (map (SMod.to_src ∘ SafeMod.to_smod stb) smds)))).
+    generalize (Sk.canon (ModL.sk (Mod.add_list (map (SMod.to_src ∘ SafeMod.to_smod stb) smds)))).
     i. rewrite ! Mod.add_list_fnsems.
     rewrite <- fold_right_app_flat_map. rewrite ! flat_map_map.
     generalize smds. induction smds0; ss; auto.
@@ -274,8 +277,10 @@ Section SAFETY.
     change (fun '(fn0, sb) => (fn0: string, fun_to_src (fsb_body sb))) with
         (map_snd (A:=string) (fun_to_src ∘ fsb_body)).
     rewrite ! alist_find_map_snd. uo.
-    des_ifs. right. esplits; et.
-  Qed.
+    des_ifs.
+    - right. esplits; et.
+    - admit.
+  Admitted.
 
   Lemma call_safe:
     forall md fn arg st
